maybe a way out of chicken and egg

dev/lf/dot_rec.v
@@ -2141,66 +2141,69 @@ Qed.
 (* ###################################################################### *)
 (** * Has member *)
 
-Inductive has_member: ctx -> var -> typ -> typ_label -> typ -> typ -> Prop :=
-| has_any : forall G x T A S U,
+Inductive has_member: nat -> ctx -> var -> typ -> typ_label -> typ -> typ -> Prop :=
+| has_any : forall n G x T A S U,
   ty_trm ty_general G empty (trm_var (avar_s x)) T ->
-  has_member_rules G x T A S U ->
-  has_member G x T A S U
-with has_member_rules: ctx -> var -> typ -> typ_label -> typ -> typ -> Prop :=
-| has_refl : forall G x A S U,
-  has_member_rules G x (typ_rcd (dec_typ A S U)) A S U
-| has_and1 : forall G x T1 T2 A S U,
-  has_member G x T1 A S U ->
-  has_member_rules G x (typ_and T1 T2) A S U
-| has_and2 : forall G x T1 T2 A S U,
-  has_member G x T2 A S U ->
-  has_member_rules G x (typ_and T1 T2) A S U
-| has_bnd : forall G x T A S U,
-  has_member G x (open_typ (in_sto x) T) A S U ->
-  has_member_rules G x (typ_bnd T) A S U
-| has_sel : forall G x y B T' A S U,
+  has_member_rules n G x T A S U ->
+  has_member n G x T A S U
+with has_member_rules: nat -> ctx -> var -> typ -> typ_label -> typ -> typ -> Prop :=
+| has_refl : forall n G x A S U,
+  has_member_rules n G x (typ_rcd (dec_typ A S U)) A S U
+| has_and1 : forall n G x T1 T2 A S U,
+  has_member n G x T1 A S U ->
+  has_member_rules n G x (typ_and T1 T2) A S U
+| has_and2 : forall n G x T1 T2 A S U,
+  has_member n G x T2 A S U ->
+  has_member_rules n G x (typ_and T1 T2) A S U
+| has_bnd : forall n G x T A S0 U,
+  has_member n G x (open_typ (in_sto x) T) A S0 U ->
+  has_member_rules (S n) G x (typ_bnd T) A S0 U
+| has_sel : forall n G x y B T' A S U,
   ty_trm ty_precise G empty (trm_var (avar_s y)) (typ_rcd (dec_typ B T' T')) ->
-  has_member G x T' A S U ->
-  has_member_rules G x (typ_sel (avar_s y) B) A S U
-| has_bot  : forall G x A S U,
-  has_member_rules G x typ_bot A S U
+  has_member n G x T' A S U ->
+  has_member_rules n G x (typ_sel (avar_s y) B) A S U
+| has_bot  : forall n G x A S U,
+  has_member_rules n G x typ_bot A S U
 .
 
 Scheme has_mut := Induction for has_member Sort Prop
 with hasr_mut := Induction for has_member_rules Sort Prop.
 Combined Scheme has_mutind from has_mut, hasr_mut.
 
-Lemma has_member_rules_inv: forall G x T A S U, has_member_rules G x T A S U ->
+Lemma has_member_rules_inv: forall n G x T A S U, has_member_rules n G x T A S U ->
   (T = typ_rcd (dec_typ A S U)) \/
   (exists T1 T2, T = typ_and T1 T2 /\
-    (has_member G x T1 A S U \/
-     has_member G x T2 A S U)) \/
-  (exists T', T = typ_bnd T' /\
-    has_member G x (open_typ (in_sto x) T') A S U) \/
+    (has_member n G x T1 A S U \/
+     has_member n G x T2 A S U)) \/
+  (exists T', T = typ_bnd T' /\ n>0 /\
+    has_member (n-1) G x (open_typ (in_sto x) T') A S U) \/
   (exists y B T', T = typ_sel (avar_s y) B /\
     ty_trm ty_precise G empty (trm_var (avar_s y)) (typ_rcd (dec_typ B T' T')) /\
-    has_member G x T' A S U) \/
+    has_member n G x T' A S U) \/
   (T = typ_bot).
 Proof.
   intros. inversion H; subst.
   - left. eauto.
   - right. left. exists T1 T2. eauto.
   - right. left. exists T1 T2. eauto.
-  - right. right. left. exists T0. eauto.
+  - right. right. left. exists T0. split; try split; eauto.
+    omega.
+    assert (Datatypes.S n0 - 1 = n0) as N by omega.
+    rewrite N. assumption.
   - right. right. right. left. exists y B T'. eauto.
   - right. right. right. right. reflexivity.
 Qed.
 
-Lemma has_member_inv: forall G x T A S U, has_member G x T A S U ->
+Lemma has_member_inv: forall n G x T A S U, has_member n G x T A S U ->
   (T = typ_rcd (dec_typ A S U)) \/
   (exists T1 T2, T = typ_and T1 T2 /\
-    (has_member G x T1 A S U \/
-     has_member G x T2 A S U)) \/
-  (exists T', T = typ_bnd T' /\
-    has_member G x (open_typ (in_sto x) T') A S U) \/
+    (has_member n G x T1 A S U \/
+     has_member n G x T2 A S U)) \/
+  (exists T', T = typ_bnd T' /\ n>0 /\
+    has_member (n-1) G x (open_typ (in_sto x) T') A S U) \/
   (exists y B T', T = typ_sel (avar_s y) B /\
     ty_trm ty_precise G empty (trm_var (avar_s y)) (typ_rcd (dec_typ B T' T')) /\
-    has_member G x T' A S U) \/
+    has_member n G x T' A S U) \/
   (T = typ_bot).
 Proof.
   intros. inversion H; subst. apply has_member_rules_inv in H1. apply H1.
@@ -2225,7 +2228,6 @@ Proof.
     assumption.
 Qed.
 
-
 Lemma rcd_typ_eq_bounds: forall T A S U,
   record_type T ->
   record_sub T (typ_rcd (dec_typ A S U)) ->
@@ -2240,12 +2242,12 @@ Proof.
 Qed.
 
 Lemma has_member_rcd_typ_sub_mut:
-  (forall G x T A S U,
-    has_member G x T A S U ->
+  (forall n G x T A S U,
+    has_member n G x T A S U ->
     record_type T ->
     record_sub T (typ_rcd (dec_typ A S U))) /\
-  (forall G x T A S U,
-    has_member_rules G x T A S U ->
+  (forall n G x T A S U,
+    has_member_rules n G x T A S U ->
     record_type T ->
     record_sub T (typ_rcd (dec_typ A S U))).
 Proof.
@@ -2262,10 +2264,10 @@ Proof.
   - destruct H as [ls H]. inversion H.
 Qed.
 
-Lemma has_member_tightness: forall G s x T ds A S U,
+Lemma has_member_tightness: forall n G s x T ds A S U,
   wf_sto G s ->
   binds x (val_new T ds) s ->
-  has_member G x (typ_bnd T) A S U ->
+  has_member n G x (typ_bnd T) A S U ->
   S = U.
 Proof.
   introv Hwf Bis Hmem.
@@ -2275,9 +2277,12 @@ Proof.
   assert (record_type (open_typ (in_sto x) T)) as Htypex. {
     apply open_record_type. assumption.
   }
-  assert (has_member G x (open_typ (in_sto x) T) A S U) as Hmemx. {
-    inversion Hmem; subst. inversion H0; subst. assumption.
+  assert (n>0 /\ has_member (n-1) G x (open_typ (in_sto x) T) A S U) as Hmemx. {
+    inversion Hmem; subst. inversion H0; subst.
+    split. omega. assert (Datatypes.S n0 -1 = n0) as B by omega.
+    rewrite B. assumption.
   }
+  destruct Hmemx as [? Hmemx].
   assert (record_sub (open_typ (in_sto x) T) (typ_rcd (dec_typ A S U))) as Hsub. {
     destruct has_member_rcd_typ_sub_mut as [HL _].
     eapply HL; eauto.
@@ -2285,12 +2290,250 @@ Proof.
   eapply rcd_typ_eq_bounds. eapply Htypex. eapply Hsub.
 Qed.
 
-Lemma has_member_covariance: forall Gs s T1 T2 x A S2 U2,
+(* ###################################################################### *)
+(** ** The substitution principle for variables *)
+
+Lemma exists_bound_restricted_by: forall x T G,
+  binds x T G ->
+  exists G', restricted_by x G G'.
+Proof.
+  intros x T.
+  apply (env_ind (fun G => binds x T G -> exists G', restricted_by x G G')).
+  - intro Bi. false. eapply binds_empty_inv; eauto.
+  - introv IH Bi.
+    apply binds_push_inv in Bi. destruct Bi as [[? ?] | [Neq Bi]].
+    + subst. eexists. apply lim_ctx with (G2:=empty).
+      rewrite concat_empty_r. reflexivity.
+    + specialize (IH Bi). destruct IH as [G' IH].
+      exists G'. inversion IH; subst. eapply lim_ctx with (G2:=G2 & x0 ~ v).
+      rewrite concat_assoc. reflexivity.
+Qed.
+
+Lemma precise_fresh_subtyp: forall Gs S U,
+  subtyp ty_precise Gs empty S U -> forall y,
+    y \notin fv_ctx_types Gs ->
+    y \notin fv_typ S ->
+    y \notin fv_typ U.
+Proof.
+  introv Hsub. dependent induction Hsub; intros; eauto;
+  try solve [simpl in H0; apply notin_union_r in H0; destruct H0; assumption].
+Qed.
+
+Lemma fresh_fv_typ: forall x y,
+  y <> x ->
+  (forall T, y \notin fv_typ T -> forall i,
+    y \notin fv_typ (open_rec_typ i (in_sto x) T)) /\
+  (forall d, y \notin fv_dec d -> forall i,
+    y \notin fv_dec (open_rec_dec i (in_sto x) d)).
+Proof.
+  intros. apply typ_mutind; intros; simpl; eauto; try solve [
+    simpl in H2; eapply notin_union_r in H2; destruct H2;
+    apply notin_union_l; eauto].
+  - simpl. unfold open_rec_avar. destruct a.
+    case_if.
+    + simpl. unfold fv_fvar. simpl. apply notin_singleton. assumption.
+    + simpl. eauto.
+    + simpl. simpl in H0. assumption.
+Qed.
+
+Lemma precise_fresh_ty_trm: forall Gs x T,
+  ty_trm ty_precise Gs empty (trm_var (avar_s x)) T -> forall y,
+    y \notin fv_ctx_types Gs -> y # Gs ->
+    y \notin fv_typ T.
+Proof.
+  introv Hty. dependent induction Hty; intros; eauto.
+  - eapply fv_ctx_types_binds; eauto.
+  - destruct (typing_implies_sto_bound Hty) as [Tx Bi].
+    assert (x <> y) as A. {
+      destruct (classicT (x = y)) as [Eq | Ne].
+      + subst. false. eapply binds_fresh_inv; eauto.
+      + assumption.
+    }
+    assert (y \notin fv_typ (typ_bnd T)) as B. {
+      eapply IHHty; eauto.
+      unfold avar_s. reflexivity.
+    }
+    eapply fresh_fv_typ; eauto.
+  - eapply precise_fresh_subtyp; eauto.
+Qed.
+
+Lemma restricted_by_first: forall x T G2 G',
+  ok (x ~ T & G2) ->
+  restricted_by x (x ~ T & G2) G' ->
+  G' = x ~ T.
+Proof.
+  introv Hok r. inversion r; subst.
+  lets Hok': (ok_restricted_by Hok r).
+  assert (empty = G1 /\ G2 = G0 /\ T = T0) as A. {
+    eapply concat_ok_eq.
+    rewrite concat_empty_l. eapply H.
+    rewrite concat_empty_l. eapply Hok.
+  }
+  destruct A as [A1 [A2 AT]]. subst.
+  rewrite concat_empty_l. reflexivity.
+Qed.
+
+Lemma subst_tight_rules: forall y S,
+   (forall m Gs G t T, ty_trm m Gs G t T -> forall s G2 x z,
+    wf_sto Gs s ->
+    G = x ~ S & G2 ->
+    ok (x ~ S & G2) ->
+    x \notin fv_ctx_types Gs -> x # Gs ->
+    ty_trm ty_precise Gs empty (trm_var (avar_s y)) (subst_typ x (in_sto y) S) ->
+    m = ty_general ->
+    t = (trm_var (avar_c z)) ->
+    ty_trm m Gs (subst_ctx x (in_sto y) G2) (subst_trm x (in_sto y) t) (subst_typ x (in_sto y) T)) /\
+  (forall m Gs G T U, subtyp m Gs G T U -> forall s G2 x,
+    wf_sto Gs s ->
+    G = x ~ S & G2 ->
+    ok (x ~ S & G2) ->
+    x \notin fv_ctx_types Gs -> x # Gs ->
+    ty_trm ty_precise Gs empty (trm_var (avar_s y)) (subst_typ x (in_sto y) S) ->
+    m = ty_general ->
+    subtyp m Gs (subst_ctx x (in_sto y) G2) (subst_typ x (in_sto y) T) (subst_typ x (in_sto y) U)).
+Proof.
+  intros y S. apply ts_mutind; intros; subst G; try subst m; try solve [false].
+  - (* ty_var_c *)
+    simpl. case_if.
+    + assert (T = S) as A. {
+        rewrite <- concat_empty_l in b. rewrite concat_assoc in b.
+        apply binds_middle_eq_inv in b. subst. reflexivity.
+        rewrite concat_empty_l. assumption.
+      }
+      subst.
+      assert ((subst_ctx x0 (in_sto y) G2)=empty & (subst_ctx x0 (in_sto y) G2)) as B. {
+        rewrite concat_empty_l. reflexivity.
+      }
+      rewrite B. apply weaken_ty_trm; eauto.
+      eapply precise_to_general_typing; eauto.
+      rewrite concat_empty_l. apply ok_map. eauto.
+    + rewrite <- concat_empty_l in b. rewrite concat_assoc in b.
+      apply binds_subst in b. rewrite concat_empty_l in b.
+      apply ty_var_c.
+      apply binds_map. assumption. assumption.
+  - (* ty_rec_intro *)
+    simpl. apply ty_rec_intro.
+    rewrite <- subst_open_commute_typ.
+    eapply H; eauto.
+  - (* ty_rec_elim *)
+    simpl. rewrite subst_open_commute_typ.
+    apply ty_rec_elim.
+    eapply H; eauto.
+  - (* ty_and_intro *)
+    simpl.
+    apply ty_and_intro; eauto.
+  - (* ty_sub *)
+    eapply ty_sub; eauto 4.
+    intro Contra. inversion Contra.
+  - (* subtyp_top *)
+    apply subtyp_top.
+  - (* subtyp_bot *)
+    apply subtyp_bot.
+  - (* subtyp_refl *)
+    apply subtyp_refl.
+  - (* subtyp_trans *)
+    eapply subtyp_trans; eauto.
+  - (* subtyp_and11 *)
+    eapply subtyp_and11; eauto.
+  - (* subtyp_and12 *)
+    eapply subtyp_and12; eauto.
+  - (* subtyp_and2 *)
+    eapply subtyp_and2; eauto.
+  - (* subtyp_fld *)
+    eapply subtyp_fld; eauto.
+  - (* subtyp_typ *)
+    eapply subtyp_typ; eauto.
+  - (* subtyp_sel2 *)
+    simpl.
+    case_if.
+    + assert (G' = x0 ~ S) as B. {
+        eapply restricted_by_first; eauto.
+      }
+      subst.
+      assert (ty_trm ty_general Gs (subst_ctx x0 (in_sto y) empty)
+        (subst_trm x0 (in_sto y) (trm_var (avar_c x0)))
+        (subst_typ x0 (in_sto y) (typ_rcd (dec_typ A S0 T)))) as Hg. {
+        eapply H; eauto.
+        rewrite concat_empty_r. reflexivity.
+        rewrite concat_empty_r. eauto.
+      }
+      simpl in Hg. rewrite If_l in Hg.
+      unfold subst_ctx in Hg. rewrite map_empty in Hg.
+      assert (avar_f (in_sto y) = (avar_s y)) as C by eauto.
+      rewrite C in Hg.
+      assert (empty & (subst_ctx x0 (in_sto y) G2) = subst_ctx x0 (in_sto y) G2) as D. {
+        rewrite concat_empty_l. reflexivity.
+      }
+      rewrite <- D. admit.
+      reflexivity.
+    + assert (exists GA2 GB2, G2 = GA2 & GB2 /\ G' = x0 ~ S & GA2) as B. {
+        admit.
+      }
+      destruct B as [GA2 [GB2 [Heq2 Heq']]]. subst.
+      eapply subtyp_sel2.
+      instantiate (1:=(subst_ctx x0 (in_sto y) GA2)). admit.
+      specialize (H s GA2 x0). simpl in H. rewrite If_r in H.
+      eapply H; eauto.
+      rewrite concat_assoc in H2. eauto.
+      assumption.
+  - (* subtyp_sel1 *)
+    admit.
+  - (* subtyp_sel2_tight *)
+    simpl. eapply subtyp_sel2_tight; eauto.
+    lets B: (precise_fresh_ty_trm t H3 H4); eauto.
+    simpl in B. apply notin_union_r in B. destruct B as [B ?].
+    assert (subst_typ x0 (in_sto y) T = T) as C. {
+      apply subst_fresh_typ.
+      assumption.
+    }
+    rewrite C. assumption.
+  - (* subtyp_sel1_tight *)
+    simpl. eapply subtyp_sel1_tight; eauto.
+    lets B: (precise_fresh_ty_trm t H3 H4); eauto.
+    simpl in B. apply notin_union_r in B. destruct B as [B ?].
+    assert (subst_typ x0 (in_sto y) T = T) as C. {
+      apply subst_fresh_typ.
+      assumption.
+    }
+    rewrite C. assumption.
+  - (* subtyp_all *)
+    simpl. apply_fresh subtyp_all as z; eauto.
+    assert (z \notin L) as FrL by eauto.
+    assert (subst_fvar x (in_sto y) (in_ctx z) = (in_ctx z)) as A. {
+      unfold subst_fvar. rewrite If_r. reflexivity. eauto.
+    }
+    rewrite <- A.
+    rewrite <- subst_open_commute_typ. rewrite <- subst_open_commute_typ.
+    assert (subst_ctx x (in_sto y) G2 & z ~ subst_typ x (in_sto y) S2 = subst_ctx x (in_sto y) (G2 & z ~ S2)) as B. {
+      unfold subst_ctx. rewrite map_concat. rewrite map_single. reflexivity.
+    }
+    rewrite B.
+    eapply H0; eauto.
+    rewrite concat_assoc. reflexivity.
+    rewrite concat_assoc. apply ok_push. assumption. eauto.
+  - (* subtyp_bnd *)
+    simpl. apply_fresh subtyp_bnd as z; eauto 4.
+    assert (z \notin L) as FrL by eauto.
+    assert (subst_fvar x (in_sto y) (in_ctx z) = (in_ctx z)) as A. {
+      unfold subst_fvar. rewrite If_r. reflexivity. eauto.
+    }
+    rewrite <- A.
+    rewrite <- subst_open_commute_typ. rewrite <- subst_open_commute_typ.
+    assert (subst_ctx x (in_sto y) G2 & z ~ typ_bnd (subst_typ x (in_sto y) T1) = subst_ctx x (in_sto y) (G2 & z ~ (typ_bnd T1))) as B. {
+      unfold subst_ctx. rewrite map_concat. rewrite map_single.
+      simpl. reflexivity.
+    }
+    rewrite B.
+    eapply H; eauto using concat_assoc.
+    rewrite concat_assoc. apply ok_push; eauto.
+Qed.
+
+Lemma has_member_covariance_zero: forall Gs s T1 T2 x A S2 U2,
   wf_sto Gs s ->
   subtyp ty_general Gs empty T1 T2 ->
   ty_trm ty_general Gs empty (trm_var (avar_s x)) T1 ->
-  has_member Gs x T2 A S2 U2 ->
-  exists S1 U1, has_member Gs x T1 A S1 U1 /\
+  has_member 0 Gs x T2 A S2 U2 ->
+  exists S1 U1, has_member 0 Gs x T1 A S1 U1 /\
                 subtyp ty_general Gs empty S2 S1 /\
                 subtyp ty_general Gs empty U1 U2.
 Proof.
@@ -2375,20 +2618,142 @@ Proof.
   - (* all *)
     inversion Hmem; subst. inversion H2; subst.
   - (* bnd *)
-    inversion Hmem; subst.
-    admit.
+    inversion Hmem; subst. inversion H2; subst.
 Qed.
 
-Lemma has_member_monotonicity: forall Gs s x T0 ds T A S U,
+Lemma has_member_covariance_aux: forall n, forall Gs s T1 T2 x A S2 U2,
+  wf_sto Gs s ->
+  subtyp ty_general Gs empty T1 T2 ->
+  ty_trm ty_general Gs empty (trm_var (avar_s x)) T1 ->
+  has_member n Gs x T2 A S2 U2 ->
+  exists S1 U1, has_member n Gs x T1 A S1 U1 /\
+                subtyp ty_general Gs empty S2 S1 /\
+                subtyp ty_general Gs empty U1 U2.
+Proof.
+  intros n. induction n.
+  eapply has_member_covariance_zero.
+  introv Hwf Hsub Hty Hmem.
+  generalize dependent U2.
+  generalize dependent S2.
+  dependent induction Hsub; subst; intros;
+  assert (@empty typ ~= @empty typ) as HE by reflexivity.
+  - (* top *)
+    inversion Hmem; subst. inversion H0.
+  - (* bot *)
+    exists S2 U2. split.
+    apply has_any. assumption. apply has_bot.
+    split; apply subtyp_refl.
+  - (* refl *)
+    exists S2 U2. eauto.
+  - (* trans *)
+    assert (ty_trm ty_general Gs empty (trm_var (avar_s x)) T) as HS. {
+      eapply ty_sub.
+      intros Hp. inversion Hp.
+      eapply Hty.
+      eassumption.
+    }
+    specialize (IHHsub2 Hwf HE HS S2 U2 Hmem).
+    destruct IHHsub2 as [S3 [U3 [Hmem3 [Hsub31 Hsub32]]]].
+    specialize (IHHsub1 Hwf HE Hty S3 U3 Hmem3).
+    destruct IHHsub1 as [S1 [U1 [Hmem1 [Hsub11 Hsub12]]]].
+    exists S1 U1. split. apply Hmem1. split; eauto.
+  - (* and11 *)
+    exists S2 U2. split.
+    inversion Hmem; subst. apply has_any. assumption. eapply has_and1. assumption.
+    split; eauto.
+  - (* and12 *)
+    exists S2 U2. split.
+    inversion Hmem; subst. apply has_any. assumption. eapply has_and2. assumption.
+    split; eauto.
+  - (* and2 *)
+    apply has_member_inv in Hmem.
+    repeat destruct Hmem as [Hmem|Hmem].
+    + inversion Hmem.
+    + destruct Hmem as [T1 [T2 [Heq [Hmem | Hmem]]]]; inversions Heq.
+      * specialize (IHHsub1 Hwf HE Hty S2 U2 Hmem). apply IHHsub1.
+      * specialize (IHHsub2 Hwf HE Hty S2 U2 Hmem). apply IHHsub2.
+    + destruct Hmem as [T1' [Heq _]]. inversion Heq.
+    + destruct Hmem as [y [B [T' [Heq _]]]]. inversion Heq.
+    + inversion Hmem.
+  - (* fld *)
+    inversion Hmem; subst. inversion H0; subst.
+  - (* typ *)
+    apply has_member_inv in Hmem.
+    repeat destruct Hmem as [Hmem|Hmem].
+    + inversions Hmem.
+      exists S1 T1. split.
+      apply has_any. assumption. apply has_refl.
+      split; assumption.
+    + destruct Hmem as [T1' [T2' [Heq _]]]. inversion Heq.
+    + destruct Hmem as [T1' [Heq _]]. inversion Heq.
+    + destruct Hmem as [y [B [T' [Heq _]]]]. inversion Heq.
+    + inversion Hmem.
+  - (* sel2 *)
+    inversion H; subst.
+    false. eapply empty_middle_inv. eassumption.
+  - (* sel1 *)
+    inversion H; subst.
+    false. eapply empty_middle_inv. eassumption.
+  - (* sel2 tight *)
+    apply has_member_inv in Hmem.
+    repeat destruct Hmem as [Hmem|Hmem].
+    + inversion Hmem.
+    + destruct Hmem as [T1' [T2' [Heq _]]]. inversion Heq.
+    + destruct Hmem as [T1' [Heq _]]. inversion Heq.
+    + destruct Hmem as [y [B [T' [Heq [Htyb Hmem]]]]]. inversions Heq.
+      assert (T' = T) as HeqT. {
+        eapply unique_tight_bounds; eassumption.
+      }
+      subst. eauto.
+    + inversion Hmem.
+  - (* sel1 tight *)
+    exists S2 U2. split.
+    eapply has_any. assumption. eapply has_sel. eassumption. eassumption.
+    eauto.
+  - (* all *)
+    inversion Hmem; subst. inversion H2; subst.
+  - (* bnd *)
+    inversion Hmem; subst. inversion H2; subst.
+    pick_fresh z. assert (z \notin L) as FrL by eauto.
+    specialize (H z FrL).
+    assert (subtyp ty_general Gs empty (open_typ (in_sto x) T1) (open_typ (in_sto x) T2)) as B. {
+      admit.
+    }
+    assert (exists S1 U1,
+        has_member n Gs x (open_typ (in_sto x) T1) A S1 U1 /\
+        subtyp ty_general Gs empty S2 S1 /\ subtyp ty_general Gs empty U1 U2) as C. {
+      eapply IHn; eauto.
+      eapply ty_rec_elim. assumption.
+    }
+    destruct C as [S1 [U1 [CA CB]]].
+    exists S1 U1. split; eauto.
+    apply has_any; eauto.
+    apply has_bnd; eauto.
+Qed.
+
+Lemma has_member_covariance: forall n Gs s T1 T2 x A S2 U2,
+  wf_sto Gs s ->
+  subtyp ty_general Gs empty T1 T2 ->
+  ty_trm ty_general Gs empty (trm_var (avar_s x)) T1 ->
+  has_member n Gs x T2 A S2 U2 ->
+  exists S1 U1, has_member n Gs x T1 A S1 U1 /\
+                subtyp ty_general Gs empty S2 S1 /\
+                subtyp ty_general Gs empty U1 U2.
+Proof.
+  introv Hwf Hsub Hty Hmem.
+  eapply has_member_covariance_aux; eauto.
+Qed.
+
+Lemma has_member_monotonicity: forall n Gs s x T0 ds T A S U,
   wf_sto Gs s ->
   binds x (val_new T0 ds) s ->
-  has_member Gs x T A S U ->
-  exists T1, has_member Gs x (typ_bnd T0) A T1 T1 /\
+  has_member n Gs x T A S U ->
+  exists n1 T1, has_member n1 Gs x (typ_bnd T0) A T1 T1 /\
              subtyp ty_general Gs empty S T1 /\
              subtyp ty_general Gs empty T1 U.
 Proof.
   introv Hwf Bis Hmem. inversion Hmem; subst.
-  generalize dependent U. generalize dependent S.
+  generalize dependent n. generalize dependent U. generalize dependent S.
   dependent induction H; intros.
   - (* var *)
     destruct (corresponding_types Hwf H).
@@ -2401,32 +2766,32 @@ Proof.
       eassumption.
     }
     subst.
-    exists U. eauto.
+    eexists. exists U. eauto.
   - (* rec_intro *)
     apply has_member_inv in Hmem.
     repeat destruct Hmem as [Hmem|Hmem].
     + inversion Hmem.
     + destruct Hmem as [T1' [T2' [Heq _]]]. inversion Heq.
     + destruct Hmem as [T1' [Heq _]]. inversions Heq.
-      apply IHty_trm; eauto.
-      inversions H0. assumption.
-      inversions H0. inversions H4. assumption.
+      inversions H0.
+      eapply IHty_trm; eauto.
+      inversions H5. assumption.
     + destruct Hmem as [y [B [T' [Heq [Htyb Hmem]]]]]. inversion Heq.
     + inversion Hmem.
   - (* rec_elim *)
-    apply IHty_trm; eauto.
-    apply has_any. assumption. apply has_bnd. assumption.
-    apply has_bnd. assumption.
+    eapply IHty_trm; eauto.
+    apply has_any. assumption. apply has_bnd. eassumption.
+    apply has_bnd. eassumption.
   - (* and_intro *)
     apply has_member_inv in Hmem.
     repeat destruct Hmem as [Hmem|Hmem].
     + inversion Hmem.
     + destruct Hmem as [T1' [T2' [Heq [Hmem | Hmem]]]];
-      inversions Heq; inversions H1; inversions H9.
-      apply IHty_trm1; eauto.
-      apply IHty_trm2; eauto. apply has_any; assumption.
-      apply IHty_trm1; eauto. apply has_any; assumption.
-      apply IHty_trm2; eauto.
+      inversions Heq; inversions H1; inversions H10.
+      eapply IHty_trm1; eauto.
+      eapply IHty_trm2; eauto. apply has_any; assumption.
+      eapply IHty_trm1; eauto. apply has_any; assumption.
+      eapply IHty_trm2; eauto.
     + destruct Hmem as [T1' [Heq _]]. inversion Heq.
     + destruct Hmem as [y [B [T' [Heq [Htyb Hmem]]]]]. inversion Heq.
     + inversion Hmem.
@@ -2435,21 +2800,21 @@ Proof.
     inversion Hmem'; subst.
     assert (@empty typ ~= @empty typ) as HE by reflexivity.
     assert (trm_var (avar_s x) = trm_var (avar_s x)) as HEx by reflexivity.
-    specialize (IHty_trm x Hwf Bis HE HEx S' U' Hmem' H4).
-    destruct IHty_trm as [T1 [Hmem1 [Hsub1 Hsub2]]].
-    exists T1. eauto.
+    specialize (IHty_trm x Hwf Bis HE HEx S' U' n Hmem' H4).
+    destruct IHty_trm as [n1 [T1 [Hmem1 [Hsub1 Hsub2]]]].
+    exists n1 T1. eauto.
 Qed.
 
 (* ###################################################################### *)
 (** * Tight bound completeness *)
 
 Lemma has_member_rcd_typ_sub2_mut:
-  (forall G x T A S U,
-    has_member G x T A S U ->
+  (forall n G x T A S U,
+    has_member n G x T A S U ->
     record_type T ->
     T = (typ_rcd (dec_typ A S U)) \/ subtyp ty_precise G empty T (typ_rcd (dec_typ A S U)))  /\
-  (forall G x T A S U,
-    has_member_rules G x T A S U ->
+  (forall n G x T A S U,
+    has_member_rules n G x T A S U ->
     record_type T ->
     T = (typ_rcd (dec_typ A S U)) \/ subtyp ty_precise G empty T (typ_rcd (dec_typ A S U))).
 Proof.
@@ -2496,12 +2861,12 @@ Lemma tight_bound_completeness: forall G s x T ds A S U,
   subtyp ty_general G empty S (typ_sel (avar_s x) A).
 Proof.
   introv Hwf Bis Hty.
-  assert (has_member G x (typ_rcd (dec_typ A S U)) A S U) as Hmem. {
+  assert (has_member 0 G x (typ_rcd (dec_typ A S U)) A S U) as Hmem. {
     apply has_any. assumption. apply has_refl.
   }
   apply has_member_monotonicity with (s:=s) (ds:=ds) (T0:=T) in Hmem.
-  destruct Hmem as [T1 [Hmem [Hsub1 Hsub2]]].
-  assert (has_member G x (open_typ (in_sto x) T) A T1 T1) as Hmemx. {
+  destruct Hmem as [n1 [T1 [Hmem [Hsub1 Hsub2]]]].
+  assert (n1>0 /\ has_member (n1-1) G x (open_typ (in_sto x) T) A T1 T1) as Hmemx. {
     apply has_member_inv in Hmem.
     repeat destruct Hmem as [Hmem|Hmem].
     + inversion Hmem.
@@ -2510,6 +2875,7 @@ Proof.
     + destruct Hmem as [y [B [T' [Heq [Htyb Hmem]]]]]. inversion Heq.
     + inversion Hmem.
   }
+  destruct Hmemx as [n0 Hmemx].
   assert (record_type T) as Htype. {
     eapply record_new_typing. eapply val_new_typing; eauto.
   }
@@ -2561,335 +2927,8 @@ Proof.
     specialize (H0 Heqm1). destruct H0. inversion H0.
 Qed.
 
-
 (* ###################################################################### *)
 (** ** The substitution principle *)
-
-Lemma exists_bound_restricted_by: forall x T G,
-  binds x T G ->
-  exists G', restricted_by x G G'.
-Proof.
-  intros x T.
-  apply (env_ind (fun G => binds x T G -> exists G', restricted_by x G G')).
-  - intro Bi. false. eapply binds_empty_inv; eauto.
-  - introv IH Bi.
-    apply binds_push_inv in Bi. destruct Bi as [[? ?] | [Neq Bi]].
-    + subst. eexists. apply lim_ctx with (G2:=empty).
-      rewrite concat_empty_r. reflexivity.
-    + specialize (IH Bi). destruct IH as [G' IH].
-      exists G'. inversion IH; subst. eapply lim_ctx with (G2:=G2 & x0 ~ v).
-      rewrite concat_assoc. reflexivity.
-Qed.
-
-Lemma precise_fresh_subtyp: forall Gs S U,
-  subtyp ty_precise Gs empty S U -> forall y,
-    y \notin fv_ctx_types Gs ->
-    y \notin fv_typ S ->
-    y \notin fv_typ U.
-Proof.
-  introv Hsub. dependent induction Hsub; intros; eauto;
-  try solve [simpl in H0; apply notin_union_r in H0; destruct H0; assumption].
-Qed.
-
-Lemma fresh_fv_typ: forall x y,
-  y <> x ->
-  (forall T, y \notin fv_typ T -> forall i,
-    y \notin fv_typ (open_rec_typ i (in_sto x) T)) /\
-  (forall d, y \notin fv_dec d -> forall i,
-    y \notin fv_dec (open_rec_dec i (in_sto x) d)).
-Proof.
-  intros. apply typ_mutind; intros; simpl; eauto; try solve [
-    simpl in H2; eapply notin_union_r in H2; destruct H2;
-    apply notin_union_l; eauto].
-  - simpl. unfold open_rec_avar. destruct a.
-    case_if.
-    + simpl. unfold fv_fvar. simpl. apply notin_singleton. assumption.
-    + simpl. eauto.
-    + simpl. simpl in H0. assumption.
-Qed.
-
-Lemma precise_fresh_ty_trm: forall Gs x T,
-  ty_trm ty_precise Gs empty (trm_var (avar_s x)) T -> forall y,
-    y \notin fv_ctx_types Gs -> y # Gs ->
-    y \notin fv_typ T.
-Proof.
-  introv Hty. dependent induction Hty; intros; eauto.
-  - eapply fv_ctx_types_binds; eauto.
-  - destruct (typing_implies_sto_bound Hty) as [Tx Bi].
-    assert (x <> y) as A. {
-      destruct (classicT (x = y)) as [Eq | Ne].
-      + subst. false. eapply binds_fresh_inv; eauto.
-      + assumption.
-    }
-    assert (y \notin fv_typ (typ_bnd T)) as B. {
-      eapply IHHty; eauto.
-      unfold avar_s. reflexivity.
-    }
-    eapply fresh_fv_typ; eauto.
-  - eapply precise_fresh_subtyp; eauto.
-Qed.
-
-Lemma restricted_by_first: forall x T G2 G',
-  ok (x ~ T & G2) ->
-  restricted_by x (x ~ T & G2) G' ->
-  G' = x ~ T.
-Proof.
-  introv Hok r. inversion r; subst.
-  lets Hok': (ok_restricted_by Hok r).
-  assert (empty = G1 /\ G2 = G0 /\ T = T0) as A. {
-    eapply concat_ok_eq.
-    rewrite concat_empty_l. eapply H.
-    rewrite concat_empty_l. eapply Hok.
-  }
-  destruct A as [A1 [A2 AT]]. subst.
-  rewrite concat_empty_l. reflexivity.
-Qed.
-
-Lemma subst_tight_rules: forall y S,
-   (forall m Gs G t T, ty_trm m Gs G t T -> forall s G2 x,
-    wf_sto Gs s ->
-    G = x ~ S & G2 ->
-    ok (x ~ S & G2) ->
-    x \notin fv_ctx_types Gs -> x # Gs ->
-    ty_trm ty_precise Gs empty (trm_var (avar_s y)) (subst_typ x (in_sto y) S) ->
-    m = ty_general ->
-    ty_trm m Gs (subst_ctx x (in_sto y) G2) (subst_trm x (in_sto y) t) (subst_typ x (in_sto y) T)) /\
-  (forall Gs G d D, ty_def Gs G d D -> forall s G2 x,
-    wf_sto Gs s ->
-    G = x ~ S & G2 ->
-    ok (x ~ S & G2) ->
-    x \notin fv_ctx_types Gs -> x # Gs ->
-    ty_trm ty_precise Gs empty (trm_var (avar_s y)) (subst_typ x (in_sto y) S) ->
-    ty_def Gs (subst_ctx x (in_sto y) G2) (subst_def x (in_sto y) d) (subst_dec x (in_sto y) D)) /\
-  (forall Gs G ds T, ty_defs Gs G ds T -> forall s G2 x,
-    wf_sto Gs s ->
-    G = x ~ S & G2 ->
-    ok (x ~ S & G2) ->
-    x \notin fv_ctx_types Gs -> x # Gs ->
-    ty_trm ty_precise Gs empty (trm_var (avar_s y)) (subst_typ x (in_sto y) S) ->
-    ty_defs Gs (subst_ctx x (in_sto y) G2) (subst_defs x (in_sto y) ds) (subst_typ x (in_sto y) T)) /\
-  (forall m Gs G T U, subtyp m Gs G T U -> forall s G2 x,
-    wf_sto Gs s ->
-    G = x ~ S & G2 ->
-    ok (x ~ S & G2) ->
-    x \notin fv_ctx_types Gs -> x # Gs ->
-    ty_trm ty_precise Gs empty (trm_var (avar_s y)) (subst_typ x (in_sto y) S) ->
-    m = ty_general ->
-    subtyp m Gs (subst_ctx x (in_sto y) G2) (subst_typ x (in_sto y) T) (subst_typ x (in_sto y) U)).
-Proof.
-  intros y S. apply rules_mutind; intros; subst G; try subst m.
-  - (* ty_var_s *)
-    simpl.
-    assert (subst_typ x0 (in_sto y) T = T) as A. {
-      apply subst_fresh_typ.
-      eapply fv_ctx_types_binds with (G:=Gs); eauto.
-    }
-    rewrite A.
-    apply ty_var_s with (T:=T); eauto.
-  - (* ty_var_c *)
-    simpl. case_if.
-    + assert (T = S) as A. {
-        rewrite <- concat_empty_l in b. rewrite concat_assoc in b.
-        apply binds_middle_eq_inv in b. subst. reflexivity.
-        rewrite concat_empty_l. assumption.
-      }
-      subst.
-      assert ((subst_ctx x0 (in_sto y) G2)=empty & (subst_ctx x0 (in_sto y) G2)) as B. {
-        rewrite concat_empty_l. reflexivity.
-      }
-      rewrite B. apply weaken_ty_trm; eauto.
-      eapply precise_to_general_typing; eauto.
-      rewrite concat_empty_l. apply ok_map. eauto.
-    + rewrite <- concat_empty_l in b. rewrite concat_assoc in b.
-      apply binds_subst in b. rewrite concat_empty_l in b.
-      apply ty_var_c.
-      apply binds_map. assumption. assumption.
-  - (* ty_all_intro *)
-    simpl.
-    apply_fresh ty_all_intro as z; eauto.
-    assert (z \notin L) as FrL by eauto.
-    assert (subst_fvar x (in_sto y) (in_ctx z) = (in_ctx z)) as A. {
-      unfold subst_fvar. rewrite If_r. reflexivity. eauto.
-    }
-    rewrite <- A.
-    rewrite <- subst_open_commute_trm. rewrite <- subst_open_commute_typ.
-    assert (subst_ctx x (in_sto y) G2 & z ~ subst_typ x (in_sto y) T = subst_ctx x (in_sto y) (G2 & z ~ T)) as B. {
-      unfold subst_ctx. rewrite map_concat. rewrite map_single. reflexivity.
-    }
-    rewrite B.
-    eapply H; eauto.
-    rewrite concat_assoc. reflexivity.
-    rewrite concat_assoc. apply ok_push. assumption. eauto.
-  - (* ty_all_elim *)
-    simpl. rewrite subst_open_commute_typ.
-    eapply ty_all_elim.
-    eapply H; eauto.
-    eapply H0; eauto.
-  - (* ty_new_intro *)
-    simpl.
-    apply_fresh ty_new_intro as z; eauto.
-    assert (z \notin L) as FrL by eauto.
-    assert (subst_fvar x (in_sto y) (in_ctx z) = (in_ctx z)) as A. {
-      unfold subst_fvar. rewrite If_r. reflexivity. eauto.
-    }
-    rewrite <- A.
-    rewrite <- subst_open_commute_typ. rewrite <- subst_open_commute_defs.
-    assert (subst_ctx x (in_sto y) G2 & z ~ subst_typ x (in_sto y) (open_typ (in_ctx z) T) = subst_ctx x (in_sto y) (G2 & z ~ open_typ (in_ctx z) T)) as B. {
-      unfold subst_ctx. rewrite map_concat. rewrite map_single. reflexivity.
-    }
-    rewrite B.
-    eapply H; eauto.
-    rewrite concat_assoc. reflexivity.
-    rewrite concat_assoc. apply ok_push. assumption. eauto.
-  - (* ty_new_elim *)
-    simpl. apply ty_new_elim.
-    eapply H; eauto.
-  - (* ty_let *)
-    simpl.
-    apply_fresh ty_let as z; eauto.
-    assert (subst_ctx x (in_sto y) G2 & z ~ subst_typ x (in_sto y) T = subst_ctx x (in_sto y) (G2 & z ~ T)) as B. {
-      unfold subst_ctx. rewrite map_concat. rewrite map_single. reflexivity.
-    }
-    rewrite B.
-    assert (subst_fvar x (in_sto y) (in_ctx z) = (in_ctx z)) as A. {
-      unfold subst_fvar. rewrite If_r. reflexivity. eauto.
-    }
-    rewrite <- A. rewrite <- subst_open_commute_trm.
-    eapply H0 with (x0:=z); eauto.
-    rewrite concat_assoc. reflexivity.
-    rewrite concat_assoc. apply ok_push. assumption. eauto.
-  - (* ty_rec_intro *)
-    simpl. apply ty_rec_intro.
-    rewrite <- subst_open_commute_typ.
-    eapply H; eauto.
-  - (* ty_rec_elim *)
-    simpl. rewrite subst_open_commute_typ.
-    apply ty_rec_elim.
-    eapply H; eauto.
-  - (* ty_and_intro *)
-    simpl.
-    apply ty_and_intro; eauto.
-  - (* ty_sub *)
-    eapply ty_sub; eauto 4.
-    intro Contra. inversion Contra.
-  - (* ty_def_typ *)
-    simpl. apply ty_def_typ; eauto.
-  - (* ty_def_trm *)
-    simpl. apply ty_def_trm; eauto.
-  - (* ty_defs_one *)
-    simpl. apply ty_defs_one; eauto.
-  - (* ty_defs_cons *)
-    simpl. apply ty_defs_cons; eauto.
-    rewrite <- subst_label_of_def.
-    apply subst_defs_hasnt. assumption.
-  - (* subtyp_top *)
-    apply subtyp_top.
-  - (* subtyp_bot *)
-    apply subtyp_bot.
-  - (* subtyp_refl *)
-    apply subtyp_refl.
-  - (* subtyp_trans *)
-    eapply subtyp_trans; eauto.
-  - (* subtyp_and11 *)
-    eapply subtyp_and11; eauto.
-  - (* subtyp_and12 *)
-    eapply subtyp_and12; eauto.
-  - (* subtyp_and2 *)
-    eapply subtyp_and2; eauto.
-  - (* subtyp_fld *)
-    eapply subtyp_fld; eauto.
-  - (* subtyp_typ *)
-    eapply subtyp_typ; eauto.
-  - (* subtyp_sel2 *)
-    simpl.
-    case_if.
-    + assert (G' = x0 ~ S) as B. {
-        eapply restricted_by_first; eauto.
-      }
-      subst.
-      assert (ty_trm ty_general Gs (subst_ctx x0 (in_sto y) empty)
-        (subst_trm x0 (in_sto y) (trm_var (avar_c x0)))
-        (subst_typ x0 (in_sto y) (typ_rcd (dec_typ A S0 T)))) as Hg. {
-        eapply H; eauto.
-        rewrite concat_empty_r. reflexivity.
-        rewrite concat_empty_r. eauto.
-      }
-      simpl in Hg. rewrite If_l in Hg.
-      unfold subst_ctx in Hg. rewrite map_empty in Hg.
-      assert (avar_f (in_sto y) = (avar_s y)) as C by eauto.
-      rewrite C in Hg.
-      assert (empty & (subst_ctx x0 (in_sto y) G2) = subst_ctx x0 (in_sto y) G2) as D. {
-        rewrite concat_empty_l. reflexivity.
-      }
-      rewrite <- D.
-      eapply weaken_subtyp.
-      eapply proj2. eapply tight_bound_completeness.
-      eassumption.
-      instantiate (1:=defs_nil). instantiate (1:=typ_top). admit.
-      eapply Hg.
-      rewrite concat_empty_l. unfold subst_ctx. apply ok_map. eauto.
-      reflexivity.
-    + assert (exists GA2 GB2, G2 = GA2 & GB2 /\ G' = x0 ~ S & GA2) as B. {
-        admit.
-      }
-      destruct B as [GA2 [GB2 [Heq2 Heq']]]. subst.
-      eapply subtyp_sel2.
-      instantiate (1:=(subst_ctx x0 (in_sto y) GA2)). admit.
-      specialize (H s GA2 x0). simpl in H. rewrite If_r in H.
-      eapply H; eauto.
-      rewrite concat_assoc in H2. eauto.
-      assumption.
-  - (* subtyp_sel1 *)
-    admit.
-  - (* subtyp_sel2_tight *)
-    simpl. eapply subtyp_sel2_tight; eauto.
-    lets B: (precise_fresh_ty_trm t H3 H4); eauto.
-    simpl in B. apply notin_union_r in B. destruct B as [B ?].
-    assert (subst_typ x0 (in_sto y) T = T) as C. {
-      apply subst_fresh_typ.
-      assumption.
-    }
-    rewrite C. assumption.
-  - (* subtyp_sel1_tight *)
-    simpl. eapply subtyp_sel1_tight; eauto.
-    lets B: (precise_fresh_ty_trm t H3 H4); eauto.
-    simpl in B. apply notin_union_r in B. destruct B as [B ?].
-    assert (subst_typ x0 (in_sto y) T = T) as C. {
-      apply subst_fresh_typ.
-      assumption.
-    }
-    rewrite C. assumption.
-  - (* subtyp_all *)
-    simpl. apply_fresh subtyp_all as z; eauto.
-    assert (z \notin L) as FrL by eauto.
-    assert (subst_fvar x (in_sto y) (in_ctx z) = (in_ctx z)) as A. {
-      unfold subst_fvar. rewrite If_r. reflexivity. eauto.
-    }
-    rewrite <- A.
-    rewrite <- subst_open_commute_typ. rewrite <- subst_open_commute_typ.
-    assert (subst_ctx x (in_sto y) G2 & z ~ subst_typ x (in_sto y) S2 = subst_ctx x (in_sto y) (G2 & z ~ S2)) as B. {
-      unfold subst_ctx. rewrite map_concat. rewrite map_single. reflexivity.
-    }
-    rewrite B.
-    eapply H0; eauto.
-    rewrite concat_assoc. reflexivity.
-    rewrite concat_assoc. apply ok_push. assumption. eauto.
-  - (* subtyp_bnd *)
-    simpl. apply_fresh subtyp_bnd as z; eauto 4.
-    assert (z \notin L) as FrL by eauto.
-    assert (subst_fvar x (in_sto y) (in_ctx z) = (in_ctx z)) as A. {
-      unfold subst_fvar. rewrite If_r. reflexivity. eauto.
-    }
-    rewrite <- A.
-    rewrite <- subst_open_commute_typ. rewrite <- subst_open_commute_typ.
-    assert (subst_ctx x (in_sto y) G2 & z ~ typ_bnd (subst_typ x (in_sto y) T1) = subst_ctx x (in_sto y) (G2 & z ~ (typ_bnd T1))) as B. {
-      unfold subst_ctx. rewrite map_concat. rewrite map_single.
-      simpl. reflexivity.
-    }
-    rewrite B.
-    eapply H; eauto using concat_assoc.
-    rewrite concat_assoc. apply ok_push; eauto.
-Qed.
 
 Lemma subst_rules: forall y S,
    (forall m Gs G t T, ty_trm m Gs G t T -> forall s G2 x,
